theories/typing.v
@@ -50,134 +50,204 @@ Definition convert_helper (sxo : option sx) t1 t2 : bool :=
   | _ => false
   end.
 
-Definition upd_label C lab :=
+Definition upd_local_label_return C loc lab ret :=
   Build_t_context
-    (tc_types_t C)
-    (tc_func_t C)
-    (tc_global C)
+    (tc_type C)
+    (tc_func C)
     (tc_table C)
     (tc_memory C)
-    (tc_local C)
+    (tc_global C)
+    (tc_elem C)
+    (tc_data C)
+    loc
     lab
-    (tc_return C).
+    ret
+    (tc_ref C).
 
-Definition plop2 C i ts :=
-  List.nth_error (tc_label C) i == Some ts.
+Definition upd_local C loc :=
+  upd_local_label_return C loc (tc_label C) (tc_return C).
+
+Definition upd_label C lab :=
+  upd_local_label_return C (tc_local C) lab (tc_return C).
+
+Definition upd_return C ret :=
+  upd_local_label_return C (tc_local C) (tc_label C) ret.
+
 
 Inductive result_typing : result -> result_type -> Prop :=
   | result_typing_values : forall vs, result_typing (result_values vs) (map typeof vs)
   | result_typing_trap : forall ts, result_typing result_trap ts
   .
 
-Inductive unop_type_agree: value_type -> unop -> Prop :=
+Inductive unop_type_agree: number_type -> unop -> Prop :=
   | Unop_i32_agree: forall op, unop_type_agree T_i32 (Unop_i op)
   | Unop_i64_agree: forall op, unop_type_agree T_i64 (Unop_i op)
   | Unop_f32_agree: forall op, unop_type_agree T_f32 (Unop_f op)
   | Unop_f64_agree: forall op, unop_type_agree T_f64 (Unop_f op)
   .
    
-Inductive binop_type_agree: value_type -> binop -> Prop :=
+Inductive binop_type_agree: number_type -> binop -> Prop :=
   | Binop_i32_agree: forall op, binop_type_agree T_i32 (Binop_i op)
   | Binop_i64_agree: forall op, binop_type_agree T_i64 (Binop_i op)
   | Binop_f32_agree: forall op, binop_type_agree T_f32 (Binop_f op)
   | Binop_f64_agree: forall op, binop_type_agree T_f64 (Binop_f op)
   .
   
-Inductive relop_type_agree: value_type -> relop -> Prop :=
+Inductive relop_type_agree: number_type -> relop -> Prop :=
   | Relop_i32_agree: forall op, relop_type_agree T_i32 (Relop_i op)
   | Relop_i64_agree: forall op, relop_type_agree T_i64 (Relop_i op)
   | Relop_f32_agree: forall op, relop_type_agree T_f32 (Relop_f op)
   | Relop_f64_agree: forall op, relop_type_agree T_f64 (Relop_f op)
   .
+
+Definition is_numeric_type (t: value_type) : bool :=
+  match t with
+  | T_num _ => true
+  | T_vec _ => true
+  | _ => false
+  end.
+
   
-Inductive be_typing : t_context -> seq basic_instruction -> function_type -> Prop :=
+
+  
+(** std-doc:
+Instructions are classified by stack types that describe how instructions manipulate the operand stack.
+
+The types describe the required input stack with operand types that an instruction pops off and
+the provided output stack with result values of types that it pushes back. Stack types are akin 
+to function types, except that they allow individual operands to be classified as ⊥ (bottom), 
+indicating that the type is unconstrained. As an auxiliary notion, an operand type t1
+matches another operand type t2, if t1 is either ⊥ or equal to t2. This is extended to stack
+types in a point-wise manner.
+
+https://www.w3.org/TR/wasm-core-2/valid/instructions.html
+ **)
+Inductive be_typing : t_context -> seq basic_instruction -> function_type -> Type :=
 | bet_const : forall C v, be_typing C [::BI_const v] (Tf [::] [::typeof v])
 | bet_unop : forall C t op,
-    unop_type_agree t op -> be_typing C [::BI_unop t op] (Tf [::t] [::t])
+    unop_type_agree t op -> be_typing C [::BI_unop t op] (Tf [::T_num t] [::T_num t])
 | bet_binop : forall C t op,
-    binop_type_agree t op -> be_typing C [::BI_binop t op] (Tf [::t; t] [::t])
-| bet_testop : forall C t op, is_int_t t -> be_typing C [::BI_testop t op] (Tf [::t] [::T_i32])
+    binop_type_agree t op -> be_typing C [::BI_binop t op] (Tf [::T_num t; T_num t] [::T_num t])
+| bet_testop : forall C t op, is_int_t t -> be_typing C [::BI_testop t op] (Tf [::T_num t] [::T_num T_i32])
 | bet_relop: forall C t op,
-    relop_type_agree t op -> be_typing C [::BI_relop t op] (Tf [::t; t] [::T_i32])
-| bet_convert : forall C t1 t2 sx, convert_helper sx t1 t2 ->
-  be_typing C [::BI_cvtop t1 CVO_convert t2 sx] (Tf [::t2] [::t1]) 
-| bet_reinterpret : forall C t1 t2, t1 <> t2 -> Nat.eqb (t_length t1) (t_length t2) ->
-  be_typing C [::BI_cvtop t1 CVO_reinterpret t2 None] (Tf [::t2] [::t1])
+    relop_type_agree t op -> be_typing C [::BI_relop t op] (Tf [::T_num t; T_num t] [::T_num T_i32])
+| bet_convert : forall C t1 t2 sx, t1 <> t2 -> convert_helper sx t1 t2 ->
+  be_typing C [::BI_cvtop t1 CVO_convert t2 sx] (Tf [::T_num t2] [::T_num t1])
+| bet_reinterpret : forall C t1 t2, t1 <> t2 -> (tnum_length t1) = (tnum_length t2) ->
+  be_typing C [::BI_cvtop t1 CVO_reinterpret t2 None] (Tf [::T_num t2] [::T_num t1])
 | bet_unreachable : forall C ts ts',
   be_typing C [::BI_unreachable] (Tf ts ts')
 | bet_nop : forall C, be_typing C [::BI_nop] (Tf [::] [::])
 | bet_drop : forall C t, be_typing C [::BI_drop] (Tf [::t] [::])
-| bet_select : forall C t, be_typing C [::BI_select] (Tf [::t; t; T_i32] [::t])
-| bet_block : forall C tn tm es,
-  let tf := Tf tn tm in
-  be_typing (upd_label C (app [::tm] (tc_label C))) es (Tf tn tm) ->
-  be_typing C [::BI_block tf es] (Tf tn tm)
-| bet_loop : forall C tn tm es,
-  be_typing (upd_label C (app [::tn] (tc_label C))) es (Tf tn tm) ->
-  be_typing C [::BI_loop (Tf tn tm) es] (Tf tn tm)
-| bet_if_wasm : forall C tn tm es1 es2,
-  be_typing (upd_label C (app [::tm] (tc_label C))) es1 (Tf tn tm) ->
-  be_typing (upd_label C (app [::tm] (tc_label C))) es2 (Tf tn tm) ->
-  be_typing C [::BI_if (Tf tn tm) es1 es2] (Tf (app tn [::T_i32]) tm)
+| bet_select_Some : forall C t, be_typing C [::BI_select (Some [::t])] (Tf [:: t; t; T_num T_i32] [::t])
+| bet_select_None : forall C t, is_numeric_type t -> be_typing C [::BI_select None] (Tf [:: t; t; T_num T_i32] [::t])
+| bet_block : forall C tb tn tm es,
+  expand_t C tb = Some (Tf tn tm) ->
+  be_typing (upd_label C ([::tm] ++ (tc_label C))) es (Tf tn tm) ->
+  be_typing C [::BI_block tb es] (Tf tn tm)
+| bet_loop : forall C tb tn tm es,
+  expand_t C tb = Some (Tf tn tm) ->
+  be_typing (upd_label C ([::tn] ++ (tc_label C))) es (Tf tn tm) ->
+  be_typing C [::BI_loop tb es] (Tf tn tm)
+| bet_if_wasm : forall C tb tn tm es1 es2,
+  expand_t C tb = Some (Tf tn tm) ->
+  be_typing (upd_label C ([::tm] ++ (tc_label C))) es1 (Tf tn tm) ->
+  be_typing (upd_label C ([::tm] ++ (tc_label C))) es2 (Tf tn tm) ->
+  be_typing C [::BI_if tb es1 es2] (Tf (tn ++ [::T_num T_i32]) tm)
 | bet_br : forall C i t1s ts t2s,
-  i < length (tc_label C) ->
-  plop2 C i ts ->
-  be_typing C [::BI_br i] (Tf (app t1s ts) t2s)
+  List.nth_error C.(tc_label) (N.to_nat i) = Some ts ->
+  be_typing C [::BI_br i] (Tf (t1s ++ ts) t2s)
 | bet_br_if : forall C i ts,
-  i < length (tc_label C) ->
-  plop2 C i ts ->
-  be_typing C [::BI_br_if i] (Tf (app ts [::T_i32]) ts)
+  List.nth_error C.(tc_label) (N.to_nat i) = Some ts ->
+  be_typing C [::BI_br_if i] (Tf (ts ++ [::T_num T_i32]) ts)
 | bet_br_table : forall C i ins ts t1s t2s,
-  all (fun i => (i < length (tc_label C)) && (plop2 C i ts)) (app ins [::i])  ->
-  be_typing C [::BI_br_table ins i] (Tf (app t1s (app ts [::T_i32])) t2s)
+  List.Forall (fun i => (List.nth_error C.(tc_label) (N.to_nat i) = Some ts)) (ins ++ [::i])  ->
+  be_typing C [::BI_br_table ins i] (Tf (t1s ++ (ts ++ [::T_num T_i32])) t2s)
 | bet_return : forall C ts t1s t2s,
   tc_return C = Some ts ->
   be_typing C [::BI_return] (Tf (app t1s ts) t2s)
 | bet_call : forall C i tf,
-  i < length (tc_func_t C) ->
-  List.nth_error (tc_func_t C) i = Some tf ->
+  List.nth_error (tc_func C) (N.to_nat i) = Some tf ->
   be_typing C [::BI_call i] tf
-| bet_call_indirect : forall C i t1s t2s,
-  i < length (tc_types_t C) ->
-  List.nth_error (tc_types_t C) i = Some (Tf t1s t2s) ->
-  tc_table C <> nil -> 
-  be_typing C [::BI_call_indirect i] (Tf (app t1s [::T_i32]) t2s)
-| bet_get_local : forall C i t,
-  i < length (tc_local C) ->
-  List.nth_error (tc_local C) i = Some t ->
-  be_typing C [::BI_get_local i] (Tf [::] [::t])
-| bet_set_local : forall C i t,
-  i < length (tc_local C) ->
-  List.nth_error (tc_local C) i = Some t ->
-  be_typing C [::BI_set_local i] (Tf [::t] [::])
-| bet_tee_local : forall C i t,
-  i < length (tc_local C) ->
-  List.nth_error (tc_local C) i = Some t ->
-  be_typing C [::BI_tee_local i] (Tf [::t] [::t])
-| bet_get_global : forall C i t,
-  i < length (tc_global C) ->
-  option_map tg_t (List.nth_error (tc_global C) i) = Some t ->
-  be_typing C [::BI_get_global i] (Tf [::] [::t])
-| bet_set_global : forall C i g t,
-  i < length (tc_global C) ->
-  List.nth_error (tc_global C) i = Some g ->  
+| bet_call_indirect : forall C x y tabtype t1s t2s,
+  List.nth_error (tc_table C) (N.to_nat x) = Some tabtype ->
+  tabtype.(tt_elem_type) = T_funcref ->
+  List.nth_error (tc_type C) (N.to_nat y) = Some (Tf t1s t2s) ->
+  be_typing C [::BI_call_indirect x y] (Tf (t1s ++ [::T_num T_i32]) t2s)
+| bet_local_get : forall C x t,
+  List.nth_error (tc_local C) (N.to_nat x) = Some t ->
+  be_typing C [::BI_local_get x] (Tf [::] [::t])
+| bet_local_set : forall C x t,
+  List.nth_error (tc_local C) (N.to_nat x) = Some t ->
+  be_typing C [::BI_local_set x] (Tf [::t] [::])
+| bet_local_tee : forall C x t,
+  List.nth_error (tc_local C) (N.to_nat x) = Some t ->
+  be_typing C [::BI_local_tee x] (Tf [::t] [::t])
+| bet_global_get : forall C x t,
+  option_map tg_t (List.nth_error (tc_global C) (N.to_nat x)) = Some t ->
+  be_typing C [::BI_global_get x] (Tf [::] [::t])
+| bet_global_set : forall C x g t,
+  List.nth_error (tc_global C) (N.to_nat x) = Some g ->  
   tg_t g = t ->
   is_mut g ->
-  be_typing C [::BI_set_global i] (Tf [::t] [::])
+  be_typing C [::BI_global_set x] (Tf [::t] [::])
+| bet_table_get : forall C x tabtype t,
+  List.nth_error (tc_table C) (N.to_nat x) = Some tabtype ->
+  tabtype.(tt_elem_type) = t ->
+  be_typing C [::BI_table_get x] (Tf [::T_num T_i32] [::T_ref t])
+| bet_table_set : forall C x tabtype t,
+  List.nth_error (tc_table C) (N.to_nat x) = Some tabtype ->
+  tabtype.(tt_elem_type) = t ->
+  be_typing C [::BI_table_set x] (Tf [::T_num T_i32; T_ref t] [::])
+| bet_table_size : forall C x tabtype,
+  List.nth_error (tc_table C) (N.to_nat x) = Some tabtype ->
+  be_typing C [::BI_table_size x] (Tf [::] [::T_num T_i32])
+| bet_table_grow : forall C x tabtype t,
+  List.nth_error (tc_table C) (N.to_nat x) = Some tabtype ->
+  tabtype.(tt_elem_type) = t ->
+  be_typing C [::BI_table_grow x] (Tf [::T_ref t; T_num T_i32] [::T_num T_i32])
+| bet_table_fill : forall C x tabtype t,
+  List.nth_error (tc_table C) (N.to_nat x) = Some tabtype ->
+  tabtype.(tt_elem_type) = t ->
+  be_typing C [::BI_table_fill x] (Tf [::T_num T_i32; T_ref t; T_num T_i32] [::T_num T_i32])
+| bet_table_copy : forall C x y tabtype1 tabtype2 t,
+  List.nth_error (tc_table C) (N.to_nat x) = Some tabtype1 ->
+  tabtype1.(tt_elem_type) = t ->
+  List.nth_error (tc_table C) (N.to_nat y) = Some tabtype2 ->
+  tabtype2.(tt_elem_type) = t ->
+  be_typing C [::BI_table_copy x y] (Tf [::T_num T_i32; T_num T_i32; T_num T_i32] [::])
+| bet_table_init : forall C x y tabtype t,
+  List.nth_error (tc_table C) (N.to_nat x) = Some tabtype ->
+  tabtype.(tt_elem_type) = t ->
+  List.nth_error (tc_elem C) (N.to_nat y) = Some t ->
+  be_typing C [::BI_table_init x y] (Tf [::T_num T_i32; T_num T_i32; T_num T_i32] [::])
+| bet_elem_drop : forall C x t,
+  List.nth_error (tc_elem C) (N.to_nat x) = Some t ->
+  be_typing C [::BI_elem_drop x] (Tf [::] [::])
 | bet_load : forall C a off tp_sx t,
   tc_memory C <> nil ->
   load_store_t_bounds a (option_projl tp_sx) t ->
-  be_typing C [::BI_load t tp_sx a off] (Tf [::T_i32] [::t])
+  be_typing C [::BI_load t tp_sx a off] (Tf [::T_num T_i32] [::T_num t])
 | bet_store : forall C a off tp t,
   tc_memory C <> nil ->
   load_store_t_bounds a tp t ->
-  be_typing C [::BI_store t tp a off] (Tf [::T_i32; t] [::]) (* two Isabelle rules have been merged here. *)
-| bet_current_memory : forall C,
+  be_typing C [::BI_store t tp a off] (Tf [::T_num T_i32; T_num t] [::])
+| bet_memory_size : forall C,
   tc_memory C <> nil ->
-  be_typing C [::BI_current_memory] (Tf [::] [::T_i32])
-| bet_grow_memory : forall C,
+  be_typing C [::BI_memory_size] (Tf [::] [::T_num T_i32])
+| bet_memory_grow : forall C,
   tc_memory C <> nil ->
-  be_typing C [::BI_grow_memory] (Tf [::T_i32] [::T_i32])
+  be_typing C [::BI_memory_grow] (Tf [::T_num T_i32] [::T_num T_i32])
+| bet_memory_fill : forall C,
+  tc_memory C <> nil ->
+  be_typing C [::BI_memory_fill] (Tf [::T_num T_i32; T_num T_i32; T_num T_i32] [::])
+| bet_memory_copy : forall C,
+  tc_memory C <> nil ->
+  be_typing C [::BI_memory_copy] (Tf [::T_num T_i32; T_num T_i32; T_num T_i32] [::])
+| bet_memory_init : forall C x,
+  tc_memory C <> nil ->
+  N.to_nat x < length (tc_data C) ->
+  be_typing C [::BI_memory_init x] (Tf [::T_num T_i32; T_num T_i32; T_num T_i32] [::])
 | bet_empty : forall C,
   be_typing C [::] (Tf [::] [::])
 | bet_composition : forall C es e t1s t2s t3s,
@@ -190,17 +260,15 @@ Inductive be_typing : t_context -> seq basic_instruction -> function_type -> Pro
 .
 
 
+(** std-doc:
+The following typing rules specify when a runtime store S is valid. A valid store must consist of
+ function, table, memory, global, and module instances that are themselves valid, relative to S.
 
-Definition upd_local C loc :=
-  Build_t_context
-    (tc_types_t C)
-    (tc_func_t C)
-    (tc_global C)
-    (tc_table C)
-    (tc_memory C)
-    loc
-    (tc_label C)
-    (tc_return C).
+To that end, each kind of instance is classified by a respective function, table, memory, or global
+ type. Module instances are classified by module contexts, which are regular contexts repurposed as
+ module types describing the index spaces defined by a module.
+https://www.w3.org/TR/wasm-core-2/appendix/properties.html#store-validity
+**)
 
 Definition upd_return C ret :=
   Build_t_context
@@ -235,14 +303,7 @@ Definition upd_local_label_return C loc lab ret :=
     lab
     ret.
 
-Definition global_agree (g : global) (tg : global_type) : bool :=
-  (tg_mut tg == g_mut g) && (tg_t tg == typeof (g_val g)).
-
-Definition globals_agree (gs : seq global) (n : nat) (tg : global_type) : bool :=
-  (n < length gs) && (option_map (fun g => global_agree g tg) (List.nth_error gs n) == Some true).
-
-Definition functions_agree (fs : seq function_closure) (n : nat) (f : function_type) : bool :=
-  (n < length fs) && (option_map cl_type (List.nth_error fs n) == Some f).
+Section Store_validity.
 
 Definition limit_match (l1 l2: limits) : bool :=
   (N.leb l2.(lim_min) l1.(lim_min)) &&
@@ -255,18 +316,21 @@ Definition limit_match (l1 l2: limits) : bool :=
         end
     end.
 
+Definition funci_agree (fs : seq function_closure) (n : funcaddr) (f : function_type) : bool :=
+  option_map cl_type (List.nth_error fs n) == Some f.
+
 Definition tab_typing (t : tableinst) (tt : table_type) : bool :=
   limit_match (Build_limits (N.of_nat (tab_size t)) t.(table_max_opt)) tt.(tt_limits).
 
-Definition tabi_agree ts (n : nat) (tab_t : table_type) : bool :=
-  (n < List.length ts) &&
-  match List.nth_error ts n with
-  | None => false
-  | Some x => tab_typing x tab_t
-  end.
-
 Definition mem_typing (m : memory) (m_t : memory_type) : bool :=
   limit_match (Build_limits (mem_size m) m.(mem_max_opt)) m_t.
+
+Definition global_agree (g : global) (tg : global_type) : bool :=
+  (tg_mut tg == g_mut g) && (tg_t tg == typeof (g_val g)).
+
+Definition globali_agree (gs : list globalinst) (n : globaladdr) (tg : global_type) : bool :=
+  option_map g_type (List.nth_error gs n) == Some tg.
+
 
 Definition memi_agree (ms : list memory) (n : nat) (mem_t : memory_type) : bool :=
   (n < length ms) &&
@@ -276,17 +340,35 @@ Definition memi_agree (ms : list memory) (n : nat) (mem_t : memory_type) : bool 
   end.
 
 
+(* TODO: figure out what's missing for elem/data/ref *)
+(** std-doc:
+https://www.w3.org/TR/wasm-core-2/appendix/properties.html#module-instances-xref-exec-runtime-syntax-moduleinst-mathit-moduleinst
+**)
 Definition inst_typing (s : store_record) (inst : instance) (C : t_context) : bool :=
-  let '{| inst_types := ts; inst_funcs := fs; inst_tab := tbs; inst_memory := ms; inst_globs := gs; |} := inst in
+  let '{| inst_types := ts; inst_funcs := fs; inst_tables := tbs; inst_mems := ms; inst_globals := gs;
+       inst_elems := es; inst_datas := ds; inst_exports := exps |} := inst in
   match C with
-  | {| tc_types_t := ts'; tc_func_t := tfs; tc_global := tgs; tc_table := tabs_t; tc_memory := mems_t; tc_local := nil; tc_label := nil; tc_return := None |} =>
+  | {| tc_type := ts'; tc_func := tfs; tc_table := tabs_t; tc_memory := mems_t; tc_global := tgs; tc_elem := nil; tc_data := nil; tc_local := nil; tc_label := nil; tc_return := None; tc_ref := nil; |} =>
     (ts == ts') &&
-    (all2 (functions_agree s.(s_funcs)) fs tfs) &&
-    (all2 (globals_agree s.(s_globals)) gs tgs) &&
+    (all2 (funci_agree s.(s_funcs)) fs tfs) &&
+    (all2 (globali_agree s.(s_globals)) gs tgs) &&
     (all2 (tabi_agree s.(s_tables)) tbs tabs_t) &&
     (all2 (memi_agree s.(s_mems)) ms mems_t)
   | _ => false
   end.
+
+
+Lemma inst_typing_expand (s: store_record) (inst: instance) (C: t_context) (tb: block_type) :
+  inst_typing s inst C ->
+  expand inst tb = expand_t C tb.
+Proof.
+  destruct tb, inst, C => //=.
+  destruct tc_elem, tc_data, tc_local, tc_label, tc_return, tc_ref => //.
+  move => Htype.
+  repeat (move/andP in Htype; destruct Htype as [Htype _]).
+  by move/eqP in Htype; subst.
+Qed.
+
 
 Inductive frame_typing: store_record -> frame -> t_context -> Prop :=
 | mk_frame_typing: forall s i tvs C f,
@@ -297,17 +379,14 @@ Inductive frame_typing: store_record -> frame -> t_context -> Prop :=
   .
 
 Lemma functions_agree_injective: forall s i t t',
-  functions_agree s i t ->
-  functions_agree s i t' ->
+  funci_agree s i t ->
+  funci_agree s i t' ->
   t = t'.
 Proof.
   move => s i t t' H1 H2.
-  unfold functions_agree in H1. unfold functions_agree in H2.
-  (*move/andP in H1. move/andP in H2.*)
-  move/andP: H1 => [_ H1].
-  move/andP: H2 => [_ H3].
-  move/eqP in H1. move/eqP in H3.
-  rewrite H3 in H1 => {H3}.
+  unfold funci_agree in *.
+  move/eqP in H1. move/eqP in H2.
+  rewrite H2 in H1 => {H2}.
   by move: H1 => [H1].
 Qed.
 
@@ -322,6 +401,15 @@ Inductive cl_typing : store_record -> function_closure -> function_type -> Prop 
     cl_typing s (FC_func_host tf h) tf
   .
 
+(** std-doc:
+Typing rules for administrative instructions are specified as follows. In addition to the context C, typing
+ of these instructions is defined under a given store S. To that end, all previous typing judgements are 
+generalized to include the store by implicitly adding S to all rules – S is never modified by the 
+pre-existing rules, but it is accessed in the extra rules for administrative instructions given below.
+
+https://www.w3.org/TR/wasm-core-2/appendix/properties.html#administrative-instructions
+**)
+
 Inductive e_typing : store_record -> t_context -> seq administrative_instruction -> function_type -> Prop :=
 | ety_a : forall s C bes tf,
   be_typing C bes tf -> e_typing s C (to_e_list bes) tf
@@ -334,11 +422,12 @@ Inductive e_typing : store_record -> t_context -> seq administrative_instruction
   e_typing s C es (Tf (ts ++ t1s) (ts ++ t2s))
 | ety_trap : forall s C tf,
   e_typing s C [::AI_trap] tf
-| ety_local : forall s C n f es ts,
-  s_typing s (Some ts) f es ts ->
-  length ts = n ->
-  e_typing s C [::AI_local n f es] (Tf [::] ts)
-| ety_invoke : forall s a C cl tf,
+| ety_ref_extern : forall s C a,
+  e_typing s C [::AI_ref_extern a] (Tf [::] [::T_ref T_externref])
+| ety_ref : forall s C a tf,
+  funci_agree s.(s_funcs) a tf ->
+  e_typing s C [::AI_ref a] (Tf [::] [::T_ref T_funcref])
+| ety_invoke : forall s (a: funcaddr) C cl tf,
   List.nth_error s.(s_funcs) a = Some cl ->
   cl_typing s cl tf ->
   e_typing s C [::AI_invoke a] tf
@@ -347,6 +436,10 @@ Inductive e_typing : store_record -> t_context -> seq administrative_instruction
   e_typing s (upd_label C ([::ts] ++ tc_label C)) es (Tf [::] t2s) ->
   length ts = n ->
   e_typing s C [::AI_label n e0s es] (Tf [::] t2s)
+| ety_local : forall s C n f es ts,
+  s_typing s (Some ts) f es ts ->
+  length ts = n ->
+  e_typing s C [::AI_local n f es] (Tf [::] ts)
 
 with s_typing : store_record -> option (seq value_type) -> frame -> seq administrative_instruction -> seq value_type -> Prop :=
 | mk_s_typing : forall s f es rs ts C C0,
@@ -373,35 +466,37 @@ Qed.
 Definition cl_type_check_single (s:store_record) (f:function_closure):=
   exists tf, cl_typing s f tf.
 
-Definition tabcl_agree (s : store_record) (tcl_index : option nat) : Prop :=
-  match tcl_index with
-  | None => True
-  | Some n => n < size s.(s_funcs)
+Definition tabcl_agree (s : store_record) (tref: reference_type) (v : value_ref) : Prop :=
+  match v with
+  | VAL_ref_null tref' => tref = tref'
+  | VAL_ref_func a => (a < length s.(s_funcs)) /\ (tref = T_funcref)
+  | VAL_ref_extern _ => tref = T_externref
   end.
 
 Definition tabsize_agree (t: tableinst) : Prop :=
-  match table_max_opt t with
+  match t.(tableinst_type).(tt_limits).(lim_max) with
   | None => True
   | Some n => tab_size t <= n
   end.
 
 Definition tab_agree (s: store_record) (t: tableinst): Prop :=
-  List.Forall (tabcl_agree s) (t.(table_data)) /\
+  List.Forall (tabcl_agree s t.(tableinst_type).(tt_elem_type)) (t.(tableinst_elem)) /\
   tabsize_agree t.
 
-Definition mem_agree (m : memory) : Prop :=
-  match (mem_max_opt m) with
+Definition mem_agree (m : meminst) : Prop :=
+  match m.(meminst_type).(lim_max) with
   | None => True
-  | Some n => N.le (mem_size m) n
+  | Some n => mem_size m <= n
   end.
 
 Definition store_typing (s : store_record) : Prop :=
   match s with
-  | Build_store_record fs tclss mss gs =>
+  | Build_store_record fs tclss mss gs es ds =>
     List.Forall (cl_type_check_single s) fs /\
     List.Forall (tab_agree s) tclss /\
     List.Forall mem_agree mss
   end.
+
 
 Inductive config_typing : store_record -> frame -> seq administrative_instruction -> seq value_type -> Prop :=
 | mk_config_typing :
@@ -409,6 +504,8 @@ Inductive config_typing : store_record -> frame -> seq administrative_instructio
   store_typing s ->
   s_typing s None f es ts ->
   config_typing s f es ts.
+
+End Store_validity.
 
 
 End Host.
